@prefix : <https://joinup.ec.europa.eu/collection/rpam/1.1.0/thesauri/constrainttaxonomy#> .
@prefix owl: <http://www.w3.org/2002/07/owl#> .
@prefix rdf: <http://www.w3.org/1999/02/22-rdf-syntax-ns#> .
@prefix xsd: <http://www.w3.org/2001/XMLSchema#> .
@prefix ccts: <http://www.unece.org/cefact#> .
@prefix rdfs: <http://www.w3.org/2000/01/rdf-schema#> .
@prefix skos: <http://www.w3.org/2004/02/skos/core#> .
@prefix dct: <http://purl.org/dc/terms/> .
@prefix skos: <http://purl.org/dc/terms/> .
@prefix skosxl: <http://www.w3.org/2008/05/skos-xl#> .
@prefix skosxl: <http://www.w3.org/2008/05/skos-xl#> .
@prefix ubl: <http://docs.oasis-open.org/ubl#> .
@base <https://joinup.ec.europa.eu/collection/rpam/1.0.0/thesauri/constrainttaxonomy#> .

<https://joinup.ec.europa.eu/collection/rpam/1.1.0/thesauri/constrainttaxonomy#> rdf:type owl:Ontology ;
                                                                               owl:versionIRI <https://joinup.ec.europa.eu/collection/rpam/1.1.0/thesauri/constrainttaxonomy#> ;
                                                                               owl:versionInfo "1.0.0"@en .

#################################################################
#    Individuals
#################################################################

# Constraints Scheme

:ConstraintsScheme rdf:type owl:NamedIndividual, skos:ConceptScheme ;
				skos:prefLabel "Constraints on the EU Power Taxonomy Data Elements."@en .

### Top Concepts 

:FINANCIAL  a owl:NamedIndividual, skos:Concept ;
			skos:prefLabel "Financial Constraint"@en ;
			skos:inScheme :ConstraintsScheme ;
			skos:definition "Expresses a financial restriction applied on a Power data element."@en .

:ADMINISTRATIVE a owl:NamedIndividual, skos:Concept ;
			skos:prefLabel "Administrative Constraint"@en ;
			skos:inScheme :ConstraintsScheme ;
			skos:definition "Limits the action to certain administrations or administrative acts."@en .

:QUANTITATIVE a owl:NamedIndividual, skos:Concept ;
			skos:prefLabel "Quantitative Constraint"@en ;
			skos:inScheme :ConstraintsScheme ;
			skos:definition "Expresses a quantitative restriction applied on a Power data element."@en .

:TEMPORAL a owl:NamedIndividual, skos:Concept ;
			skos:prefLabel "Temporal Constraint"@en ;
			skos:inScheme :ConstraintsScheme ;
			skos:definition "Expresses a temporal restriction applied on a Power data element. E.g. and end date, a start date, a period, a quantity of years, months, weeks, days, hours."@en .

:DOCUMENTARY a owl:NamedIndividual, skos:Concept ;
			skos:prefLabel "Documentary Constraint"@en ;
			skos:inScheme :ConstraintsScheme ;
			skos:definition "Expresses a restriction about a type of document, record or evidence required by the Service Provider."@en .

:ABOVE_AGE a owl:NamedIndividual, skos:Concept ;
			skos:prefLabel "Above Age"@en ;
			skos:inScheme :ConstraintsScheme ;
			skos:hasTopConcept :QUANTITATIVE ;
			skos:broader :QUANTITATIVE ;
			skosxl:prefLabel :AboveAgeType;
			skos:definition "The minimum age required by the Service Provider."@en .

:GET a owl:NamedIndividual, skos:Concept ;
			skos:prefLabel "Greater Or Equal Than"@en ;
			skos:inScheme :ConstraintsScheme ;
			skos:hasTopConcept :QUANTITATIVE ;
			skos:broader :QUANTITATIVE ;
			skosxl:prefLabel :GreaterOREqualThanType ;
			skos:definition "The minimum quantity required by the Service Provider."@en .

:LET a owl:NamedIndividual, skos:Concept ;
			skos:prefLabel "Lesser Or Equal Than"@en ;
			skos:inScheme :ConstraintsScheme ;
			skos:hasTopConcept :QUANTITATIVE ;
			skos:broader :QUANTITATIVE ;
			skosxl:prefLabel :LesserOrEqualThanType ;
			skos:definition "The maximum quantity required by the Service Provider."@en .

:MIN_AMOUNT a owl:NamedIndividual, skos:Concept ;
			skos:prefLabel "Minimum Amount"@en ;
			skos:inScheme :ConstraintsScheme ;
			skos:hasTopConcept :FINANCIAL ;
			skos:broader :FINANCIAL ;
			skosxl:prefLabel :AmountType ;
			skos:definition "The minimum amount required by the Service Provider in a financial operation. The currency should be identified."@en .

:MAX_AMOUNT a owl:NamedIndividual, skos:Concept ;
			skos:prefLabel "Maximum Amount"@en ;
			skos:inScheme :ConstraintsScheme ;
			skos:hasTopConcept :FINANCIAL ;
			skos:broader :FINANCIAL;
			skosxl:prefLabel :AmountType ;
			skos:definition "The maximum amount required by the Service Provider. The currency should be identified."@en .

:MIN_DATE a owl:NamedIndividual, skos:Concept ;
			skos:prefLabel "Minimum Date"@en ;
			skos:inScheme :ConstraintsScheme ;
			skos:hasTopConcept :TEMPORAL;
			skos:broader :TEMPORAL ;
			skosxl:prefLabel :DateType ;
			skos:definition "The minimum date specified by the Service Provider."@en .

:MAX_DATE a owl:NamedIndividual, skos:Concept ;
			skos:prefLabel "Maximum Date"@en ;
			skos:inScheme :ConstraintsScheme ;
			skos:hasTopConcept :TEMPORAL;
			skos:broader :TEMPORAL ;
			skosxl:prefLabel :DateType ;
			skos:definition "The maximum date specified by the Service Provider."@en .

:START_END_DATE a owl:NamedIndividual, skos:Concept ;
			skos:prefLabel "Start Date End Date"@en ;
			skos:inScheme :ConstraintsScheme ;
			skos:hasTopConcept :TEMPORAL;
			skos:broader :TEMPORAL ;
			skosxl:prefLabel :PeriodStartEndDateType ;
			skos:definition "The period of time specified by the Service Provider as a start date and an end date."@en .

:START_DATE_LAPSE a owl:NamedIndividual, skos:Concept ;
			skos:prefLabel "Start Date And Lapse"@en ;
			skos:inScheme :ConstraintsScheme ;
			skos:hasTopConcept :TEMPORAL;
			skos:broader :TEMPORAL ;
			skosxl:prefLabel :PeriodLapseType ;
			skos:definition "The period of time specified by the Service Provider as a start date and a quantity of years, months, weeks, etc."@en .

:EVIDENCE_TYPE a owl:NamedIndividual, skos:Concept ;
			skos:prefLabel "Evidence Type"@en ;
			skos:inScheme :ConstraintsScheme ;
			skos:hasTopConcept :DOCUMENTARY ;
			skos:broader :DOCUMENTARY ;
			skosxl:prefLabel :EvidenceType ;
			skos:definition "Type of evidence."@en .

:EVIDENCE_SCHEME_VERSION a owl:NamedIndividual, skos:Concept ;
			skos:prefLabel "Evidence Scheme Version"@en ;
			skos:inScheme :ConstraintsScheme ;
			skos:hasTopConcept :DOCUMENTARY ;
			skos:broader :DOCUMENTARY ;
			skosxl:prefLabel :EvidenceSchemeVersionType ;
			skos:definition "Version number of the scheme defining a type of evidence."@en .

### Branches and leaves

:ADMINISTRATION_LEVEL a owl:NamedIndividual, skos:Concept ;
			skos:prefLabel "Public Administration Level"@en ;
			skos:inScheme :ConstraintsScheme ;
			skos:definition "The level of the Public Administration for which the Mandatee has the power of acting on behalf of the Mandator"@en ;
			skos:broader :ADMINISTRATIVE ;
			skos:hasTopConcept :ADMINISTRATIVE .

:MAX_CONTRACT_THRESHOLD a owl:NamedIndividual, skos:Concept ;
			skos:prefLabel "Maximum contract value threshold"@en ;
			skos:inScheme :ConstraintsScheme ;
			skos:definition "The maximum amount for contracts signed by a Mandatee representing a Natural or Legal Person"@en ;
			skos:broader :FINANCIAL ;
			skos:hasTopConcept :FINANCIAL .

