@prefix : <https://joinup.ec.europa.eu/collection/rpam/1.0.0/emandateresponse#> .
@prefix : <http://data.europa.eu/RPaM/ontology#> .
@prefix owl: <http://www.w3.org/2002/07/owl#> .
@prefix rdf: <http://www.w3.org/1999/02/22-rdf-syntax-ns#> .
@prefix ubl: <http://docs.oasis-open.org/ubl#> .
@prefix xml: <http://www.w3.org/XML/1998/namespace> .
@prefix xsd: <http://www.w3.org/2001/XMLSchema#> .
@prefix ccev: <https://joinup.ec.europa.eu/collection/semic/ccev/2.0.3/ontology#> .
@prefix ccts: <http://www.unece.org/cefact#> .
@prefix rdfs: <http://www.w3.org/2000/01/rdf-schema#> .
@prefix skos: <http://www.w3.org/2004/02/skos/core#> .
@prefix cpsvap: <http://data.europa.eu/m8g/cpsvap#> .
@prefix person: <http://www.w3.org/ns/person#> .
@prefix foaf: <http://xmlns.com/foaf/0.1/> .
@base <https://joinup.ec.europa.eu/collection/rpam/1.0.0/emandateresponse#> .

<https://joinup.ec.europa.eu/collection/rpam/1.0.0/emandateresponse#> rdf:type owl:Ontology ;
                                        owl:versionIRI <https://joinup.ec.europa.eu/collection/rpam/1.0.0/emandateresponse> .

#################################################################
#    Object Properties
#################################################################

:provides rdf:type owl:ObjectProperty, owl:TransitiveProperty ;
      rdfs:range :Mandate ;
      rdfs:label "provides" ;
      skos:definition "The response of and eMandate, as a result, provides a Mandate."@en .

:documents rdf:type owl:ObjectProperty ,
                   owl:TransitiveProperty ;
          rdfs:domain :eMandateResponse ;
          rdfs:range :Exception ;
          rdfs:label "documents"@en ;
#         skos:definition "...."@en .

#################################################################
#    Data properties -- DELETE and COMPLETE
#################################################################

###  http://data.europa.eu/RPaM/ontology#hasCurrentDelegationLevel
#:currentDelegationLevel rdf:type owl:DatatypeProperty ;
#                           rdfs:domain :Power ;
#                           rdfs:range xsd:positiveInteger ;
#                          rdfs:label "Current Delegation Level"@en ;
#                          skos:definition "The current level of the delegation of the power, if the power can be delegated. E.g. 0 (never delegated), 1 (delegated once), 2 (delegated twice), etc."@en .

#################################################################
#    Classes
#################################################################

:eMandateResponse rdf:type owl:Class ;
          rdfs:label "eMandate Response"@en ;
          skos:definition "An eDocument provided by an eMandate Registry containing the data about an eMandate."@en .

     owl:subClassOf [
                        a owl:Restriction ;
                        owl:someValuesFrom :Mandate ;
                        owl:onProperty :provides
                        ] ;
     owl:subClassOf [
                        a owl:Restriction ;
                        owl:someValuesFrom :Exception ;
                        owl:onProperty :documents
                        ] .  

:Exception rdf:type owl:Class ;
       rdfs:label "Exception"@en ;
       skos:definition "Describes the possible causes of the exceptions."@en .                          

###### DELETE ######

#:Mandatee rdf:type owl:Class ;
#          owl:rdfs:subClassOf foaf:Agent ;
#          rdfs:label "Mandatee"@en ;
#          skos:definition "Natural or legal person that acts on behalf of another natural or legal person."@en .

#:Mandator rdf:type owl:Class ;
#          owl:rdfs:subClassOf foaf:Agent ;
#          rdfs:label "Mandator"@en ;
#          skos:definition "Person who needs an activity executed in his name; creator of the mandate."@en .

#:Power rdf:type owl:Class ;
#       rdfs:label "Power"@en ;
#       skos:definition "The capacity to act on its own behalf."@en .

