@prefix : <https://joinup.ec.europa.eu/collection/rpam/1.0.0/epowerresponse#> .
@prefix : <http://data.europa.eu/RPaM/ontology#> .
@prefix owl: <http://www.w3.org/2002/07/owl#> .
@prefix rdf: <http://www.w3.org/1999/02/22-rdf-syntax-ns#> .
@prefix ubl: <http://docs.oasis-open.org/ubl#> .
@prefix xml: <http://www.w3.org/XML/1998/namespace> .
@prefix xsd: <http://www.w3.org/2001/XMLSchema#> .
@prefix ccev: <https://joinup.ec.europa.eu/collection/semic/ccev/2.0.3/ontology#> .
@prefix ccts: <http://www.unece.org/cefact#> .
@prefix rdfs: <http://www.w3.org/2000/01/rdf-schema#> .
@prefix skos: <http://www.w3.org/2004/02/skos/core#> .
@prefix cpsvap: <http://data.europa.eu/m8g/cpsvap#> .
@prefix person: <http://www.w3.org/ns/person#> .
@prefix foaf: <http://xmlns.com/foaf/0.1/> .
@base @prefix : <https://joinup.ec.europa.eu/collection/rpam/1.0.0/epowerresponse#> .

@prefix : <https://joinup.ec.europa.eu/collection/rpam/1.0.0/epowerresponse#>  rdf:type owl:Ontology ;
                                        owl:versionIRI @prefix : <https://joinup.ec.europa.eu/collection/rpam/1.0.0/epowerresponse#> .

#################################################################
#    Object Properties
#################################################################

:hasMandator rdf:type owl:ObjectProperty ;
      rdfs:range :Mandator ;
      rdfs:label "has Mandator" ;
      skos:definition "The role of a natural person or a legal person as a mandator or a mandatee."@en .

:hasPower rdf:type owl:ObjectProperty ,
                   owl:TransitiveProperty ;
          rdfs:domain :Mandator, :Mandatee ;
          rdfs:range :Power ;
          rdfs:label "has Power"@en ;
          skos:definition "The capacity to act on ownself (power) or on behalf of another (representation power)."@en .

:roleOf rdf:type owl:ObjectProperty ,
               owl:FunctionalProperty ;
      rdfs:domain :Mandatee ,
                  :Mandator ;
      rdfs:range foaf:Agent ;
      rdfs:label "role Of" ;
      skos:definition "The role of a natural person or a legal person as a mandator or a mandatee."@en .

:satisfiesSPInformationRequirements rdf:type owl:ObjectProperty ;
                          rdfs:domain :Mandator ;
                          rdfs:range ccev:Criterion ;
                          rdfs:label "satisfies SP Information Requirements"@en ;
                          skos:definition "A mandator or mandatee satisfies the constraints set by the Service Provider."@en .

:includesEvidence rdf:type owl:ObjectProperty ;
                          rdfs:domain :ePowerResponse;
                          rdfs:range ccev:Evidence;
                          rdfs:label "includes Evidence."@en ;
                          skos:definition "Evidence(s) provided by the user (mandator) to access a cross-border Service Provider system."@en .

:validityPeriod rdf:type owl:ObjectProperty ,
                            owl:FunctionalProperty ;
                   rdfs:domain :Power ;
                   rdfs:range ubl:Period ;
                   rdfs:label "has Validity Period"@en .

:geospatialConstraint rdf:type owl:ObjectProperty ;
                         rdfs:domain :Power ;
                         # e.g. a NUTS code
                         rdfs:range skos:Concept ;
                         rdfs:label "Geospatial Constraint"@en ;
                         skos:definition "Common power constraint establishing the geographical or spatial scope of the power."@en .

:ID rdf:type owl:ObjectProperty, owl:FunctionalProperty ;
                       rdfs:domain :Mandatee, :Mandator, :Power ;
                       rdfs:range ccts:Identifier ;
                       rdfs:label "The identifier of a Mandator, a mandatee or a power"@en .

:statusType rdf:type owl:ObjectProperty ;
               rdfs:domain :Power ;
               rdfs:range skos:Concept ;
               rdfs:label "Status Type"@en ;
               skos:definition "The current status of the power, e.g. ACTIVE, REVOKED, TEMPORALITY_SUSPENDED, etc."@en .

:financialThresholdConstraint rdf:type owl:ObjectProperty ;
                              rdfs:domain :Power ;
                              rdfs:range ubl:Amount ;
                              rdfs:label "Financial Threshold Constraint"@en ;
                              skos:definition "Common power constraint limiting the power to a financial threshold."@en .

#################################################################
#    Data properties
#################################################################

###  http://data.europa.eu/RPaM/ontology#hasCurrentDelegationLevel
:currentDelegationLevel rdf:type owl:DatatypeProperty ;
                           rdfs:domain :Power ;
                           rdfs:range xsd:positiveInteger ;
                           rdfs:label "Current Delegation Level"@en ;
                           skos:definition "The current level of the delegation of the power, if the power can be delegated. E.g. 0 (never delegated), 1 (delegated once), 2 (delegated twice), etc."@en .

#################################################################
#    Classes
#################################################################

:ePoweresponse rdf:type owl:Class ;
          rdfs:label "ePower Response"@en ;
          skos:definition "An eDocument provided by an eMandate Registry containing the data about the powers of user acting on its own behalf."@en .

:Mandator rdf:type owl:Class ;
          owl:rdfs:subClassOf foaf:Agent ;
          rdfs:label "Mandator"@en ;
          skos:definition "Person who needs an activity executed in his name; creator of the mandate."@en .

:Power rdf:type owl:Class ;
       rdfs:label "Power"@en ;
       skos:definition "The capacity to act on its own behalf."@en .

