@prefix : <https://joinup.ec.europa.eu/collection/rpam/1.1.0/ontology#> .
@prefix owl: <http://www.w3.org/2002/07/owl#> .
@prefix rdf: <http://www.w3.org/1999/02/22-rdf-syntax-ns#> .
@prefix ubl: <http://docs.oasis-open.org/ubl#> .
@prefix xml: <http://www.w3.org/XML/1998/namespace> .
@prefix xsd: <http://www.w3.org/2001/XMLSchema#> .
@prefix ccev: <https://joinup.ec.europa.eu/collection/semic/ccev/2.0.3/ontology#> .
@prefix ccts: <http://www.unece.org/cefact#> .
@prefix rdfs: <http://www.w3.org/2000/01/rdf-schema#> .
@prefix skos: <http://www.w3.org/2004/02/skos/core#> .
@prefix foaf: <http://xmlns.com/foaf/0.1/> .
@base <http://data.europa.eu/RPaM/ontology#> .

<https://joinup.ec.europa.eu/collection/rpam/1.1.0/ontology#> rdf:type owl:Ontology ;
                                        owl:versionIRI <https://joinup.ec.europa.eu/collection/rpam/1.1.0/ontology> .

#################################################################
#    Object Properties
#################################################################

:id rdf:type owl:ObjectProperty, owl:FunctionalProperty ;
                       rdfs:domain :Mandate, :Empowerment, :Mandatee, :Mandator;
                       rdfs:range ccts:Identifier ;
                       rdfs:label "The identifier of a mandate, mandator, mandatee or empowerment."@en .

:mandatorConstraint  rdf:type owl:ObjectProperty, owl:FunctionalProperty ;
                     rdfs:label "power Use Constraint"@en ;
                     skos:definition "Constraint(s) imposed on how mandators with delegated powers may use a power."@en ;
                     skos:example "Geospatial, temporal, financial, contractual, etc. constraints or possible combinations of these."@en .

:mandateeConstraint  rdf:type owl:ObjectProperty, owl:FunctionalProperty ;
                     rdfs:label "mandateeConstraint"@en ;
                     skos:definition "Constraint(s) imposed on how mandators with delegated powers may use a power."@en ;
                     skos:example "Geospatial, temporal, financial, contractual, etc. constraints or possible combinations of these."@en .

:empowerment rdf:type owl:ObjectProperty, owl:FunctionalProperty;
          rdfs:label "hasEmpowerment" ;
          rdfs:definition "The assignment of one power and restrictions on its use to one or more mandatees ." .

:lifeSpan rdf:type owl:ObjectProperty ;
          rdfs:domain :Mandate ;
          rdfs:range ubl:Period ;
          rdfs:label "hasLifeSpan"@en ;
          skos:definition "The dates of creation and striking-off of a mandate in the eMandate Registry."@en .
                                 
:mandator  rdf:type owl:ObjectProperty, owl:FunctionalProperty ;
          rdfs:label "hasMandator" ;
          rdfs:definition "The person that empowers." .

:mandatee  rdf:type owl:ObjectProperty, owl:FunctionalProperty ;
          rdfs:label "hasMandatee" ;
          rdfs:definition "The person being empowered." .

:powerType  rdf:type owl:ObjectProperty ;
          rdfs:domain :Empowerment ;
          rdfs:range :EUPowerTaxonomy ;
          rdfs:label "hasPowerType."@en ;
          skos:definition "The yype of power provided through the empowerment of Mandatee by a Mandator." .

:statusType rdf:type owl:ObjectProperty ;
               rdfs:domain :Power ;
               rdfs:range skos:Concept ;
               rdfs:label "hasStatusType"@en ;
               skos:definition "The status of the empowerment." .


#################################################################
#    Data properties
#################################################################

:delegationLevel rdf:type owl:DatatypeProperty , owl:FunctionalProperty ;
                           rdfs:domain :Empowerment ;
                           rdfs:range xsd:integer ;
                           rdfs:label "currentDelegationLevel"@en ;
                           skos:definition "The number of times that a power has been assigned by a mandatee to another mandatee."@en .

#################################################################
#    Classes
#################################################################

:Empowerment rdf:type owl:Class ;
       rdfs:label "Empowerment"@en ;
       skos:definition "The specification of how one mandator assigns one power, and possible constraints on its use, to one or more Mandatees." ;
       owl:subClassOf [
                             a owl:Restriction ;
                             owl:someValuesFrom skos:Concept ;
                             owl:onProperty :powerType
                           ] ;
     
       owl:subClassOf [
                             a owl:Restriction ;
                             owl:someValuesFrom ccev:Criterion ;
                             owl:onProperty :mandatorConstraint
                           ] ;
       owl:subClassOf [
                             a owl:Restriction ;
                             owl:someValuesFrom ccev:Criterion ;
                             owl:onProperty :mandateeConstraint
                    ] ;

      owl:subClassOf [
                             a owl:Restriction ;
                             owl:someValuesFrom :Mandatee ;
                             owl:onProperty :mandatee
                           ] .                          

:Mandate rdf:type owl:Class ;
       rdfs:label "Mandate"@en ;
       skos:definition "Collection of empowerments."@en ;

      owl:subClassOf [
                             a owl:Restriction ;
                             owl:allValuesFrom :Mandator ;
                             owl:onProperty :mandator
                           ] ;
       owl:subClassOf [
                             a owl:Restriction ;
                             owl:someValuesFrom :Empowerment ;
                             owl:onProperty :empowerment
                           ] .
      
:Mandatee rdf:type owl:Class ;
          owl:rdfs:subClassOf foaf:Agent ;
          rdfs:label "Mandatee"@en ;
          skos:definition "Natural or legal person that acts on behalf of another natural or legal person."@en ;
          owl:subClassOf [
                            a owl:Restriction ;
                            owl:someValuesFrom ccev:Criterion  ;
                            owl:onProperty :constraint ;
                            skos:definition "Constraint(s) imposed on how mandatees may use a power."@en ;
                            skos:example "Geospatial, temporal, financial, contractual, etc. constraints or possible combinations of these."@en 
                         ] .

:Mandator rdf:type owl:Class ;
          owl:rdfs:subClassOf foaf:Agent ;
          rdfs:label "Mandator"@en ;
          skos:definition "Person who needs an activity executed in his name; creator of the mandate."@en ;
          
          .


