@prefix :        <https://joinup.ec.europa.eu/collection/rpam/1.0.0/thesauri/status#> .
@prefix adms:    <http://www.w3.org/ns/adms#>.
@prefix foaf:    <http://xmlns.com/foaf/0.1/>.
@prefix grddl:   <http://www.w3.org/2003/g/data-view#> .
@prefix dct:     <http://purl.org/dc/terms/> .
@prefix rdf:     <http://www.w3.org/1999/02/22-rdf-syntax-ns#> .
@prefix owl:     <http://www.w3.org/2002/07/owl#> .
@prefix skosxl:  <http://www.w3.org/2008/05/skos-xl#> .
@prefix xsd:     <http://www.w3.org/2001/XMLSchema#> .
@prefix skos:  	 <http://www.w3.org/2004/02/skos/core#> .
@prefix rdfs:    <http://www.w3.org/2000/01/rdf-schema#> .
@prefix dc:      <http://purl.org/dc/elements/1.1/> .
@prefix dcterms: <http://purl.org/dc/terms/> .
@prefix dcat:    <http://www.w3.org/ns/dcat#> .
@base            <https://joinup.ec.europa.eu/collection/rpam/1.0.0/thesauri/status#> .

#metadata

<https://joinup.ec.europa.eu/collection/rpam/1.0.0/thesauri/status#> a owl:Ontology, adms:Asset;
	owl:versionIRI <https://joinup.ec.europa.eu/collection/rpam/1.0.0/thesauri/status#> ;
	dcterms:title "Powers Status Taxonomy"@en;
	skos:description "Definition of the powers used in the European Union to act on behalf of another person in front of a service, e.g. an online service supplied by a public administration."@en ;
	#dcterms:description "The Powers Taxonomy ...."@en;
	dcterms:created "2018-10-10"^^xsd:date;
	#vann:preferredNamespacePrefix "rpam";
	#foaf:homepage <http://...>;
	#dcterms:publisher [foaf:name "European Commission"];
	#dcterms:creator [foaf:name "Core Public Service Working Group"; foaf:homepage <http://joinup.ec.europa.eu/asset/core_public_service/document/core-public-service-working-group>.];
	dcterms:type <http://purl.org/adms/assettype/Ontology>;
	dcterms:status <http://purl.org/adms/status/UnderDevelopment> ;
	dct:description "A Data Set with one mandates conformat to the RPaM Ontology specification, supplied from an eMandate Registry in response to the request of a Service Provider (SP)."@en ,
	                "BEWARE that this Ontology is an ongoing development"@en ;
	dct:publisher "European Commission, ISA2 Programme"@en ;
	dct:creator "everis, Spain, S.L.U"@en ;
	dcat:distribution [
	        dcat:accessURL <https://github.com/everis-rpam> ;
	        skos:note "The URL GitHub Repository to download this file."@en ;
	        dcat:downloadURL <https://github.com/everis-rpam/RPaM-Ontology/blob/v1.1.0/03-Syntax_Bindings/OWL-DL-TTL/rpam/thesauri/EU_Power_Status_Taxonomy.ttl>                                         
	] .
#skos:ConceptScheme

:EU_RPaM_Status_Taxonomy a skos:ConceptScheme ;
	dct:created "2018-10-25T11:16:28.041+02:00"^^xsd:dateTime ;
	skosxl:prefLabel :EU_POWER_STATUS .

:EU_POWER_STATUS a skosxl:Label ;
	skosxl:literalForm "EU RPaM Status Taxonomy"@en .

:POWER_STATUS a skos:Concept ;
	dct:created "2018-10-25T11:17:04.836+02:00"^^xsd:dateTime ;
	skos:inScheme :EU_RPaM_Status_Taxonomy ;
	skos:topConceptOf :EU_RPaM_Status_Taxonomy ;
	skosxl:prefLabel [
						a skosxl:Label ;
						skosxl:literalForm "Power Status"@en 
					 ] .

#skos:Concepts


:APPROVED a skos:Concept ;
	dct:created "2018-10-25T11:17:18.096+02:00"^^xsd:dateTime ;
	skos:broader :ePower_Status ;
	skos:definition "The ePower Request has been accepted and the Mandatee can already act on behalf of the Mandator."@en ;
	skos:inScheme :EU_RPaM_Status_Taxonomy ;
	skosxl:prefLabel [
						a skosxl:Label ;
						skosxl:literalForm "Approved"@en 
					 ] .

:CONFIRMED a skos:Concept ;
	dct:created "2018-10-25T11:27:13.611+02:00"^^xsd:dateTime ;
	skos:broader :APPROVED ;
	skos:definition "A confirmation (acceptance) from the Mandatee is required once the power has been approved by the PS."@en ;
	skos:inScheme :EU_RPaM_Status_Taxonomy ;
	skosxl:prefLabel [
						a skosxl:Label ;
						skosxl:literalForm "Confirmed"@en 
					 ] .

:CONSUMED a skos:Concept ;
	skos:broader :APPROVED ;
	skos:definition "The power has been consumed."@en ;
	skos:inScheme :EU_RPaM_Status_Taxonomy ;
	skosxl:prefLabel [
						a skosxl:Label ;
						skosxl:literalForm "Consumed"@en 
					 ] .

:EU_RPaM_STATUS_TAXONOMY a skos:Concept ;
	dct:created "2018-10-25T11:16:28.041+02:00"^^xsd:dateTime ;
	skosxl:prefLabel [
						a skosxl:Label ;
						skosxl:literalForm "EU RPaM Status Taxonomy"@en 
					 ] .

:EXPIRED a skos:Concept ;
	dct:created "2018-10-25T11:28:23.210+02:00"^^xsd:dateTime ;
	skos:broader :APPROVED ;
	skos:definition "The power has expired and is no longer valid."@en ;
	skos:inScheme :EU_RPaM_Status_Taxonomy ;
	skosxl:prefLabel [
						a skosxl:Label ;
						skosxl:literalForm "Expired"@en 
					 ] .

:EXTENDED a skos:Concept ;
	dct:created "2018-10-25T11:29:15.744+02:00"^^xsd:dateTime ;
	skos:broader :APPROVED ;
	skos:definition "The Mandator may extend the period of validity of the power as long as it does not exceed the period established by the legislation in force."@en ;
	skos:inScheme :EU_RPaM_Status_Taxonomy ;
	skosxl:prefLabel [
						a skosxl:Label ;
						skosxl:literalForm "Extended"@en 
					 ] .

:PENDING a skos:Concept ;
	dct:created "2018-10-25T11:17:50.082+02:00"^^xsd:dateTime ;
	skos:broader :ePower_Status ;
	skos:definition "The ePower is pending of resolution."@en ;
	skos:inScheme :EU_RPaM_Status_Taxonomy ;
	skosxl:prefLabel [
						a skosxl:Label ;
						skosxl:literalForm "Pending"@en 
					 ] .

:RENOUNCED a skos:Concept ;
	dct:created "2018-10-25T11:34:26.402+02:00"^^xsd:dateTime ;
	skos:broader :APPROVED ;
	skos:definition "The Mandatee may renounce the power that has been assigned to him/her."@en ;
	skos:inScheme :EU_RPaM_Status_Taxonomy ;
	skosxl:prefLabel [
						a skosxl:Label ;
						skosxl:literalForm "Renounced"@en 
					 ] .

:REVOKED a skos:Concept ;
	dct:created "2018-10-25T11:32:16.098+02:00"^^xsd:dateTime ;
	skos:broader :APPROVED ;
	skos:definition "A Mandator may decide at any time whether or not to revoque the power(s) that have been assigned to the Mandatee."@en ;
	skos:inScheme :EU_RPaM_Status_Taxonomy ;
	skosxl:prefLabel [
						a skosxl:Label ;
						skosxl:literalForm "Revoked"@en 
					 ] .


:STRUCK_OFF_MANDATE a skos:Concept ;
	dct:created "2019-02-17T14:18:16"^^xsd:dateTime ;
	skos:broader :ePower_Status ;
	skos:definition "The power is no longer valid because the mandate where it was defined has been struck off."@en ;
	skos:inScheme :EU_RPaM_Status_Taxonomy ;
	skosxl:prefLabel [
						a skosxl:Label ;
						skosxl:literalForm "Revoked"@en 
					 ] .
