@prefix : <https://joinup.ec.europa.eu/collection/rpam/1.0.0/thesauri/power-ir-ded#> .
@prefix owl: <http://www.w3.org/2002/07/owl#> .
@prefix rdf: <http://www.w3.org/1999/02/22-rdf-syntax-ns#> .
@prefix xml: <http://www.w3.org/XML/1998/namespace> .
@prefix xsd: <http://www.w3.org/2001/XMLSchema#> .
@prefix ccts: <http://www.unece.org/cefact#> .
@prefix rdfs: <http://www.w3.org/2000/01/rdf-schema#> .
@prefix skos: <http://www.w3.org/2004/02/skos/core#> .
@prefix dct: <http://purl.org/dc/terms/> .
@prefix skos: <http://purl.org/dc/terms/> .
@prefix skosxl: <http://www.w3.org/2008/05/skos-xl#> .
@prefix vcard: <http://www.w3.org/2006/vcard/ns#> .
@prefix foaf: <http://xmlns.com/foaf/0.1/> .
@base <https://joinup.ec.europa.eu/collection/rpam/1.0.0/thesauri/power-ir-ded#> .
<https://joinup.ec.europa.eu/collection/rpam/1.0/thesauri/power-ir-ded#> rdf:type owl:Ontology ;
                                                                               owl:versionIRI <https://joinup.ec.europa.eu/collection/rpam/1.0.0/thesauri/power-ir-ded> ;
                                                                               owl:versionInfo "1.0.0" .
#    Individuals

# PIR Elements
:PowerIRScheme rdf:type owl:NamedIndividual, skos:ConceptScheme ;
				skos:prefLabel "EU Powers Taxonomy - Information Requirements Data Elements." .
:NP a owl:NamedIndividual, skos:Concept ;
			skos:prefLabel "Natural Person"@en ;
			skos:inScheme :PowerIRScheme ;
			skosxl:prefLabel :NaturalPersonType ;
			skos:definition "Top concept grouping information requirement data elements related to persons (i.e. natural persons)"@en .
:LP a owl:NamedIndividual, skos:Concept ;
			skos:prefLabel "Legal Person"@en ;
			skos:inScheme :PowerIRScheme ;
			skosxl:prefLabel :LegalPersonType ;
			skos:definition "Top concept grouping information requirement data elements related to organisations (i.e. legal entities)"@en . 
:DOCUMENTARY a owl:NamedIndividual, skos:Concept ;
			skos:prefLabel "Documentary"@en ;
			skos:inScheme :PowerIRScheme ;
			skos:definition "Top concept grouping information requirement data elements related to documents, records, evidences, evidence templates, etc."@en .
# Natural Person attributes
:NP_ID a owl:NamedIndividual, skos:Concept ;
			skos:prefLabel "Natural Person ID Number"@en ;
			skos:inScheme :PowerIRScheme ;
			skos:hasTopConcept :NP ;
			skos:broader :NP ;
			skosxl:prefLabel :NaturalPersonIDType;
			skos:definition "The identification number of the person."@en .
:GIVEN_NAME a owl:NamedIndividual, skos:Concept ;
			skos:prefLabel "Given Name"@en ;
			skos:inScheme :PowerIRScheme ;
			skos:hasTopConcept :NP ;
			skosxl:prefLabel :GivenNameType;
			skos:definition "The given name of the person."@en .
:FAMILY_NAME a owl:NamedIndividual, skos:Concept ;
			skos:prefLabel "Family Name"@en ;
			skos:inScheme :PowerIRScheme ;
			skos:hasTopConcept :NP ;
			skos:broader :NP ;
			skosxl:prefLabel :FamilyNameType;
			skos:definition "The family name of the person."@en .
:FIRST_RESIDENCE_ADDRESS a owl:NamedIndividual, skos:Concept ;
			skos:prefLabel "First Residence Address"@en ;
			skos:inScheme :PowerIRScheme ;
			skos:hasTopConcept :NP ;
			skos:broader :NP ;
			skosxl:prefLabel :NaturalPersonAddressType;
			skos:definition "The first residence address of the person."@en .
:DATE_OF_BIRTH a owl:NamedIndividual, skos:Concept ;
			skos:prefLabel "Date Of Birth"@en ;
			skos:inScheme :PowerIRScheme ;
			skos:hasTopConcept :NP ;
			skos:broader :NP ;
			skosxl:prefLabel :DateOfBirthType ;
			skos:definition "The date when the person was born."@en .			
:PLACE_OF_BIRTH a owl:NamedIndividual, skos:Concept ;
			skos:prefLabel "Place Of Birth"@en ;
			skos:inScheme :PowerIRScheme ;
			skos:hasTopConcept :NP ;
			skos:broader :NP ;
			skosxl:prefLabel :PlaceOfBirthType ;
			skos:definition "The place where the natural person was born."@en .			
:AGE a owl:NamedIndividual, skos:Concept ;
			skos:prefLabel "Age"@en ;
			skos:inScheme :PowerIRScheme ;
			skos:hasTopConcept :NP ;
			skos:broader :NP ;
			skosxl:prefLabel :AgeType ;
			skos:definition "The age of the person expressed as the positive integer number of years."@en .
:CITIZENSHIP a owl:NamedIndividual, skos:Concept ;
			skos:prefLabel "Citizenship"@en ;
			skos:inScheme :PowerIRScheme ;
			skos:hasTopConcept :NP ;
			skos:broader :NP ;
			skosxl:prefLabel :CitizenshipType ;
			skos:definition "The citizenship of the person."@en .
:GENDER a owl:NamedIndividual, skos:Concept ;
			skos:prefLabel "Gender"@en ;
			skos:inScheme :PowerIRScheme ;
			skos:hasTopConcept :NP ;
			skos:broader :NP ; 
			skosxl:prefLabel :GenderType ;
			skos:definition "The gender of the person."@en .
# Legal Person attributes
:LP_ID a owl:NamedIndividual, skos:Concept ;
			skos:prefLabel "Legal Person Identifier"@en ;
			skos:inScheme :PowerIRScheme ;
			skos:hasTopConcept :LP ;
			skos:broader :LP ;
			skosxl:prefLabel :LegalPersonIDType ;
			skos:definition "The identifier number of the organisation. E.g. the BRIS EUID, a LEI number, etc."@en .
:REGISTERED_NAME a owl:NamedIndividual, skos:Concept ;
			skos:prefLabel "Registered Name"@en ;
			skos:inScheme :PowerIRScheme ;
			skos:hasTopConcept :LP ;
			skos:broader :LP ;
			skosxl:prefLabel :RegisteredNameType ;
			skos:definition "The name of the organisation as registered in an official registry."@en .		
:REGISTERED_ADDRESS a owl:NamedIndividual, skos:Concept ;
			skos:prefLabel "Registered Address"@en ;
			skos:inScheme :PowerIRScheme ;
			skos:hasTopConcept :LP ;
			skos:broader :LP ;
			skosxl:prefLabel :RegisteredAddressType ;
			skos:definition "The address of the organisation as registered in an official registry."@en .					
:LEGAL_FORM a owl:NamedIndividual, skos:Concept ;
			skos:prefLabel "Legal Form"@en ;
			skos:inScheme :PowerIRScheme ;
			skos:hasTopConcept :LP ;
			skos:broader :LP ;
			skosxl:prefLabel :LegalFormType ;
			skos:definition "The legal form of the organisation. E.g. Limited company, Cooperative, etc."@en .
# Documentary IR Data Elements
:EVIDENCE_ID a owl:NamedIndividual, skos:Concept ;
			skos:prefLabel "Evidence Identifier"@en ;
			skos:inScheme :PowerIRScheme ;
			skos:hasTopConcept :DOCUMENTARY ;
			skos:broader :DOCUMENTARY ;
			skosxl:prefLabel :EvidenceIdentifierType ;
			skos:definition "The identifier of the evidence (e.g. an EU RPaM eMandate)"@en .
# PIR Element Data Types
## Natural Person PIR Element Data Types
:NaturalPersonType a skosxl:Label ;
	rdf:type skosxl:Label ;
	dct:type foaf:Person ;
    rdfs:label "NaturalPersonType"@en ;
    skosxl:literalForm "Natural Person Type"@en ;
    skos:definition "The type of information element representing a natural person." .
:NaturalPersonIDType a skosxl:Label ;
	rdf:type skosxl:Label ;
	dct:type ccts:Identifier ;
    rdfs:label "NaturalPersonIDType"@en ;
    skosxl:literalForm "Natural Person ID Number Type"@en ;
    skos:definition "The type of information element representing the identifier number of a natural person." .
:GivenNameType a  skosxl:Label ;
	rdf:type skosxl:Label ;
	dct:type ccts:Text ;
    rdfs:label "GivenNameType"@en ;
    skosxl:literalForm "Given Name Type"@en ;
    skos:definition "The type of information element representing the given name of a natural person." .	
 :FamilyNameType a  skosxl:Label ;
	rdf:type skosxl:Label ;
	dct:type ccts:Text ;
    rdfs:label "FamilyNameType"@en ;
    skosxl:literalForm "Family Name Type"@en ;
    skos:definition "The type of information element representing the family name of a natural person." .		
:NaturalPersonAddressType a skosxl:Label ;
	rdf:type skosxl:Label ;
	dct:type vcard:Address ;
    rdfs:label "NaturalPersonAddressType"@en ;
    skosxl:literalForm "Natural Person Address Type"@en ;
    skos:definition "The type of the information element representing the first residence of a natural person." .	
:DateOfBirthType a skosxl:Label ;
	rdf:type skosxl:Label ;
	dct:type xsd:Date ;
    rdfs:label "DateOfBirthType"@en ;
    skosxl:literalForm "Date of Birth Type"@en ;
    skos:definition "The type of the information element representing the date when a natural person was born." .	
:PlaceOfBirthType a skosxl:Label ;
	rdf:type skosxl:Label ;
	dct:type vcard:Address ;
    rdfs:label "PlaceOfBirthType"@en ;
    skosxl:literalForm "Place of Birth Type"@en ;
    skos:definition "The type of the information element representing the place where a natural person was born." .	
:AgeType a skosxl:Label ;
	rdf:type skosxl:Label ;
	dct:type ccts:Quantity ;
    rdfs:label "AgeType"@en ;
    skosxl:literalForm "Age Type"@en ;
    skos:definition "The type of the information element representing the age of a natural person, e.g. the integer positive number of years." .	
:CitizenshipType a skosxl:Label ;
	rdf:type skosxl:Label ;
	dct:type skos:Concept ;
    rdfs:label "CitizenshipType"@en ;
    skosxl:literalForm "Citizenship Type"@en ;
    skos:definition "The type of the information element representing the citizenship of a natural person, e.g. a country code." .
:GenderType a skosxl:Label ;
	rdf:type skosxl:Label ;
	dct:type vcard:Gender ;
    rdfs:label "GenderType"@en ;
    skosxl:literalForm "Gender Type"@en ;
    skos:definition "The type of the information element representing the gender of a natural person." .
## Legal Person PIR Element Data Types
:LegalPersonType a skosxl:Label ;
	rdf:type skosxl:Label ;
	dct:type foaf:LegalEntity;
    rdfs:label "LegalPersonType"@en ;
    skosxl:literalForm "Legal Person Type"@en ;
    skos:definition "The type of information element representing a legal person." .
:LegalPersonIDType a skosxl:Label ;
	rdf:type skosxl:Label ;
	dct:type ccts:Identifier ;
    rdfs:label "LegalPersonIDType"@en ;
    skosxl:literalForm "Legal Person ID Number Type"@en ;
    skos:definition "The type of information element representing the identifier number of a legal person." .	
 :RegisteredNameType a  skosxl:Label ;
	rdf:type skosxl:Label ;
	dct:type ccts:Text ;
    rdfs:label "RegisteredNameType"@en ;
    skosxl:literalForm "Family Name Type"@en ;
    skos:definition "The name of a legal person as registered in an official Registry." .	
 :RegisteredAddressType a  skosxl:Label ;
	rdf:type skosxl:Label ;
	dct:type vcard:Address ;
    rdfs:label "RegisteredAddressType"@en ;
    skosxl:literalForm "Registered Address Type"@en ;
    skos:definition "The address of a legal person as registered in an official Registry." .	
:LegalFormType a  skosxl:Label ;
	rdf:type skosxl:Label ;
	dct:type skos:Concept ;
    rdfs:label "LegalFormType"@en ;
    skosxl:literalForm "Legal Form Type"@en ;
    skos:definition "The legal form of legal person as registered in an official Registry." ;
    skos:example "Limited Company"@en ;
    skos:example "Sociedad Limitada"@es .	
# Documentary Data Elements Types
:EvidenceIdentifierType a skosxl:Label ;
	rdf:type skosxl:Label ;
	dct:type foaf:Person ;
    rdfs:label "EvidenceIdentifierType"@en ;
    skosxl:literalForm "EvidenceIdentifierType"@en ;
    skos:definition "The type of information element representing the identifier of an evidence."@en .
