@prefix : <https://joinup.ec.europa.eu/collection/rpam/1.0.0/ontology#> .
@prefix owl: <http://www.w3.org/2002/07/owl#> .
@prefix rdf: <http://www.w3.org/1999/02/22-rdf-syntax-ns#> .
@prefix ubl: <http://docs.oasis-open.org/ubl#> .
@prefix xml: <http://www.w3.org/XML/1998/namespace> .
@prefix xsd: <http://www.w3.org/2001/XMLSchema#> .
@prefix ccev: <https://joinup.ec.europa.eu/collection/semic/ccev/2.0.3/ontology#> .
@prefix ccts: <http://www.unece.org/cefact#> .
@prefix rdfs: <http://www.w3.org/2000/01/rdf-schema#> .
@prefix skos: <http://www.w3.org/2004/02/skos/core#> .
@prefix foaf: <http://xmlns.com/foaf/0.1/> .
@base <http://data.europa.eu/RPaM/ontology#> .

<https://joinup.ec.europa.eu/collection/rpam/1.0.0/ontology#> rdf:type owl:Ontology ;
                                        owl:versionIRI <https://joinup.ec.europa.eu/collection/rpam/1.0.0/ontology> .

#################################################################
#    Object Properties
#################################################################

:hasPower rdf:type owl:ObjectProperty ;
          rdfs:domain :Mandate ;
          rdfs:range :Power ;
          rdfs:label "has Power"@en ;
          skos:definition "The Powers in a Mandate that a Mandator assigns to a Mandatee."@en .

:powerOf  rdf:type owl:ObjectProperty ;
          rdfs:domain :Power ;
          rdfs:range :Mandator ;
          rdfs:label "power of" ;
          rdfs:definition "The Powers of a Mandator that he may be assigned to a Mandatee" 
          .

:lifeSpan rdf:type owl:ObjectProperty ;
          rdfs:domain :Mandate ;
          rdfs:range ubl:Period ;
          rdfs:label "has lifeSpan"@en ;
          skos:definition "The dates of creation and striking-off of the  Mandate in the eMandate Registry."@en .

:typeOf   rdf:type owl:ObjectProperty ;
          rdfs:domain :Power ;
          rdfs:range :EUPowerTaxonomy ;
          rdfs:label "has type of power"@en ;
          skos:definition "The Type of Power provided through the empowerment of Mandatee by a Mandator"
          .

:assignedTo rdf:type owl:ObjectProperty ;
              rdfs:domain :Power ;
              rdfs:range :Mandatee ;
              rdfs:label "assigned To"@en ;
              skos:definition "The Powers in a Mandate that a Mandatee receives from a Mandator."@en .

:satisfiesRequirements rdf:type owl:ObjectProperty ;
                          rdfs:domain :Mandatee ,
                                      :Mandator ;
                          rdfs:range ccev:Criterion ;
                          rdfs:label "satisfies Service Provider Information Requirements"@en ;
                          skos:definition "A mandator or mandatee satisfies the constraints set by the Service Provider."@en .

:geospatialConstraint rdf:type owl:ObjectProperty ;
                         rdfs:domain :Power ;
                         rdfs:range :GeolocationConstraint ;
                         rdfs:label "Geospatial Constraint"@en .


:ID rdf:type owl:ObjectProperty, owl:FunctionalProperty ;
                       rdfs:domain :Mandate, :Mandatee, :Mandator, :Power ;
                       rdfs:range ccts:Identifier ;
                       rdfs:label "The identifier of a Mandator, a mandatee or a power"@en .


:statusType rdf:type owl:ObjectProperty ;
               rdfs:domain :Power ;
               rdfs:range skos:Concept ;
               rdfs:label "Status Type"@en .

:validityPeriodConstraint rdf:type owl:ObjectProperty ,
                            owl:FunctionalProperty ;
                          rdfs:domain :Power ;
                          rdfs:range ubl:Period ;
                          rdfs:label "has Validity Period"@en .

:financialThresholdConstraint rdf:type owl:ObjectProperty ;
                                    rdfs:domain :Power ;
                                    rdfs:range ubl:Amount ;
                                    rdfs:label "Financial Threshold Constraint"@en .

#################################################################
#    Data properties
#################################################################

###  http://data.europa.eu/RPaM/ontology#hasCurrentDelegationLevel
:currentDelegationLevel rdf:type owl:DatatypeProperty ;
                           rdfs:domain :Power ;
                           rdfs:range xsd:positiveInteger ;
                           rdfs:label "Current Delegation Level"@en .

#################################################################
#    Classes
#################################################################

:Mandate rdf:type owl:Class ;
       rdfs:label "Mandate"@en ;
       skos:definition "The result of the empowerment of a Mandatee by a Mandator, i.e. the expression of which powers have been assigned by a Person (the Mandator) to another Person (the Mandatee), for certain purposes, for a certain period of time, under certain possible circumstances, etc."@en .

:Mandatee rdf:type owl:Class ;
          owl:rdfs:subClassOf foaf:Agent ;
          rdfs:label "Mandatee"@en ;
          skos:definition "Natural or legal person that acts on behalf of another natural or legal person."@en .

:Mandator rdf:type owl:Class ;
          owl:rdfs:subClassOf foaf:Agent ;
          rdfs:label "Mandator"@en ;
          skos:definition "Person who needs an activity executed in his name; creator of the mandate."@en .

:Power rdf:type owl:Class ;
       rdfs:label "Power"@en ;
       skos:definition "The capacity to act on its own behalf."@en .